New mechanism for heap_lang substitutions.
It is based on type classes and can it be tuned by providing
instances, for example, instances can be provided to mark that
certain expressions are closed.

barrier/barrier.v
@@ -1,5 +1,10 @@
-From heap_lang Require Export notation.
+From heap_lang Require Export substitution notation.
 
-Definition newchan := (λ: "", ref '0)%L.
-Definition signal := (λ: "x", "x" <- '1)%L.
-Definition wait := (rec: "wait" "x" :=if: !"x" = '1 then '() else "wait" "x")%L.
+Definition newchan : val := λ: "", ref '0.
+Definition signal : val := λ: "x", "x" <- '1.
+Definition wait : val :=
+  rec: "wait" "x" := if: !"x" = '1 then '() else "wait" "x".
+
+Instance newchan_closed : Closed newchan. Proof. solve_closed. Qed.
+Instance signal_closed : Closed signal. Proof. solve_closed. Qed.
+Instance wait_closed : Closed wait. Proof. solve_closed. Qed.
