heap_lang/derived.v
@@ -16,20 +16,20 @@ Implicit Types P Q : iProp heap_lang Σ.
 Implicit Types Φ : val → iProp heap_lang Σ.
 
 (** Proof rules for the sugar *)
-Lemma wp_lam' E x ef e v Φ :
+Lemma wp_lam E x ef e v Φ :
   to_val e = Some v →
   ▷ || subst ef x v @ E {{ Φ }} ⊑ || App (Lam x ef) e @ E {{ Φ }}.
-Proof. intros. by rewrite -wp_rec' ?subst_empty. Qed.
+Proof. intros. by rewrite -wp_rec ?subst_empty. Qed.
 
-Lemma wp_let' E x e1 e2 v Φ :
+Lemma wp_let E x e1 e2 v Φ :
   to_val e1 = Some v →
   ▷ || subst e2 x v @ E {{ Φ }} ⊑ || Let x e1 e2 @ E {{ Φ }}.
-Proof. apply wp_lam'. Qed.
+Proof. apply wp_lam. Qed.
 
 Lemma wp_seq E e1 e2 v Φ :
   to_val e1 = Some v →
   ▷ || e2 @ E {{ Φ }} ⊑ || Seq e1 e2 @ E {{ Φ }}.
-Proof. intros ?. rewrite -wp_let' // subst_empty //. Qed.
+Proof. intros ?. rewrite -wp_let // subst_empty //. Qed.
 
 Lemma wp_skip E Φ : ▷ Φ (LitV LitUnit) ⊑ || Skip @ E {{ Φ }}.
 Proof. rewrite -wp_seq // -wp_value //. Qed.
