heap_lang/lifting.v
@@ -84,7 +84,7 @@ Qed.
 
 (* For the lemmas involving substitution, we only derive a preliminary version.
    The final version is defined in substitution.v. *)
-Lemma wp_rec' E f x e1 e2 v Φ :
+Lemma wp_rec E f x e1 e2 v Φ :
   to_val e2 = Some v →
   ▷ || subst (subst e1 f (RecV f x e1)) x v @ E {{ Φ }}
   ⊑ || App (Rec f x e1) e2 @ E {{ Φ }}.
@@ -93,6 +93,13 @@ Proof.
     (subst (subst e1 f (RecV f x e1)) x v) None) ?right_id //=;
     intros; inv_step; eauto.
 Qed.
+
+Lemma wp_rec' E f x erec v1 e2 v2 Φ :
+  v1 = RecV f x erec →
+  to_val e2 = Some v2 →
+  ▷ || subst (subst erec f v1) x v2 @ E {{ Φ }}
+  ⊑ || App (of_val v1) e2 @ E {{ Φ }}.
+Proof. intros ->. apply wp_rec. Qed.
 
 Lemma wp_un_op E op l l' Φ :
   un_op_eval op l = Some l' →
@@ -140,7 +147,7 @@ Proof.
     ?right_id -?wp_value //; intros; inv_step; eauto.
 Qed.
 
-Lemma wp_case_inl' E e0 v0 x1 e1 x2 e2 Φ :
+Lemma wp_case_inl E e0 v0 x1 e1 x2 e2 Φ :
   to_val e0 = Some v0 →
   ▷ || subst e1 x1 v0 @ E {{ Φ }} ⊑ || Case (InjL e0) x1 e1 x2 e2 @ E {{ Φ }}.
 Proof.
@@ -148,7 +155,7 @@ Proof.
     (subst e1 x1 v0) None) ?right_id //; intros; inv_step; eauto.
 Qed.
 
-Lemma wp_case_inr' E e0 v0 x1 e1 x2 e2 Φ :
+Lemma wp_case_inr E e0 v0 x1 e1 x2 e2 Φ :
   to_val e0 = Some v0 →
   ▷ || subst e2 x2 v0 @ E {{ Φ }} ⊑ || Case (InjR e0) x1 e1 x2 e2 @ E {{ Φ }}.
 Proof.
